Foundation/ProvabilityLogic/Arithmetic.lean
@@ -20,6 +20,20 @@ lemma provable_iff :
     ProvabilityLogic T U ⊢! A ↔ ∀ f : T.StandardRealization, U ⊢!. f A := by
   simp [ArithmeticTheory.ProvabilityLogic]
 
+lemma mdp : ProvabilityLogic T U ⊢! A ➝ B → ProvabilityLogic T U ⊢! A → ProvabilityLogic T U ⊢! B := by
+  simp only [provable_iff];
+  intro hAB hA f;
+  replace hAB : U ⊢!. f A ➝ f B := hAB f;
+  replace hA : U ⊢!. f A := hA f;
+  cl_prover [hAB, hA]
+
+instance : Entailment.ModusPonens (ProvabilityLogic T U) := ⟨by
+  rintro A B ⟨hA⟩ ⟨hB⟩;
+  constructor;
+  simp only [←Modal.Logic.iff_provable] at hA hB ⊢;
+  apply mdp hA hB;
+⟩
+
 end ArithmeticTheory.ProvabilityLogic
 
 end LO.FirstOrder
